PFPL/ch6.v
@@ -1,4 +1,5 @@
 Require Import Env.
+Require Import TransitiveClosure.
 
 Inductive Ty :=
         | t_num   : Ty
@@ -18,11 +19,402 @@ Definition TEnv := Env Ty.
 Inductive TYPE (env : TEnv) : Exp -> Ty -> Prop :=
 	| ty_env (v : Var) (t : Ty): (InEnv v t env) -> TYPE env (var v) t
 	| ty_num (n : Num) : TYPE env (num n) t_num
-	| ty_lambda (def body : Exp) (ty tbody : Ty) :
+	| ty_lambda (body : Exp) (ty tbody : Ty) :
 		TYPE (ty :: env) body tbody ->
 		TYPE env (lambda ty body) (t_arrow ty tbody)
 	| ty_app (f x : Exp) (t1 t2 : Ty) :
 		TYPE env f (t_arrow t1 t2) ->
 		TYPE env x t1 ->
 		TYPE env (app f x) t2.
+
+
+Lemma unicity
+	(env: TEnv) (e : Exp) (t1 t2 : Ty)
+	(Ht1 : TYPE env e t1)
+	(Ht2 : TYPE env e t2)
+	: t1 = t2.
+Proof.
+  revert t2 Ht2.
+  induction Ht1; intros; inversion Ht2; subst; try congruence.
+  f_equal. apply IHHt1. assumption.
+  
+  apply IHHt1_1 in H1.
+  apply IHHt1_2 in H3.
+  congruence.
+Qed.
+
+Fixpoint raise (e : Exp) (a b : nat) :=
+ match e with
+ | var v      => var (raise' a b v)
+ | num n      => num n
+ | lambda t x => lambda t (raise x a (S b))
+ | app f x    => app (raise f a b) (raise x a b)
+ end.
+
+Lemma raise_0_id (e : Exp) (n : nat) :
+	raise e 0 n = e.
+Proof.
+ revert n.
+ induction e; intros; simpl; try (rewrite IHe1, IHe2); try reflexivity.
+ unfold raise, raise'.
+ destruct (ge_dec v n); auto.
+ rewrite IHe. reflexivity.
+Qed. 
+
+Lemma weakening_insert
+        (env : TEnv) (e : Exp) (te tvi : Ty) (vi : Var) :
+        TYPE env e te ->
+        TYPE (insert env vi tvi) (raise e 1 vi) te.
+ intros Hte.
+ revert vi tvi.
+ induction Hte; intros; try solve [constructor; auto].
+ apply ty_env.
+ unfold raise', InEnv, getEnv in *.
+ destruct (ge_dec v vi).
+ apply get_insert_ge; assumption.
+ apply get_insert_lt. assumption.
+ omega.
+
+ apply ty_lambda; fold raise.
+ rewrite <- uninsert; auto.
+ eapply ty_app; fold raise; auto.
+Qed.
+
+Lemma weakening_cons
+	(env : TEnv) (e : Exp) (te : Ty) tv : 
+	TYPE env e te ->
+	TYPE (tv :: env) (raise e 1 0) te.
+Proof.
+ rewrite <- insert_0.
+ apply weakening_insert.
+Qed.
+
+
+
+Fixpoint subst (e e' : Exp) (v : Var) :=
+ match e with
+ | var v'     => subst' v v' var e'
+ | num n      => num n
+ | lambda t x => lambda t (subst x (raise e' 1 0) (S v))
+ | app    f x => app (subst f e' v) (subst x e' v)
+ end.
+
+Lemma minus_n_1 v:
+      S v - 1 = v.
+ simpl. rewrite minus_n_O. reflexivity.
+Qed.
+
+Lemma substitution_ix env x t t' e e':
+      TYPE (insert env x t) e'             t' ->
+      TYPE env              e              t  ->
+      x <= length env                         ->
+      TYPE env              (subst e' e x) t'.
+Proof.
+ intros Ht' Ht Hlen.
+ remember (insert env x t) as ENV.
+ revert env x t e HeqENV Ht Hlen.
+ induction Ht'; intros; try solve [constructor; auto].
+   unfold subst, subst'.
+   destruct (eq_nat_dec x v); subst.
+    apply InEnv_insert in H. subst. assumption.
+   destruct (lt_dec x v); subst.
+    apply ty_env.
+    destruct v. omega.
+     rewrite minus_n_1.
+     eapply insert_minus1; eassumption.
+   apply ty_env. eapply insert_pre; try eassumption; try omega.
+
+ simpl; subst; apply ty_lambda.
+ eapply IHHt'. reflexivity.
+ apply weakening_cons; assumption.
+ simpl. omega.
+ 
+ simpl; subst; eapply ty_app.
+ eapply IHHt'1. reflexivity. assumption. assumption.
+ eapply IHHt'2. reflexivity. assumption. assumption.
+Qed.
+
+
+Lemma substitution env t t' e e':
+      TYPE (t :: env)       e'             t' ->
+      TYPE env              e              t  ->
+      TYPE env              (subst e' e 0) t'.
+Proof.
+ intros.
+ eapply substitution_ix; try rewrite insert_0; try eassumption; try omega.
+Qed.
+
+Lemma decomposition env x t t' e e':
+      TYPE env              (subst e' e x) t' ->
+      TYPE env              e              t  ->
+      x <= length env                         ->
+      TYPE (insert env x t) e'             t'.
+Proof.
+ intros Hsub Ht Hlen.
+ revert env x t t' e Hsub Ht Hlen.
+ induction e'; intros.
+ simpl in Hsub; unfold subst' in Hsub.
+  apply ty_env.
+  destruct (eq_nat_dec x v).
+    replace t with t' by (eapply unicity; eassumption).
+    replace v with x  by assumption.
+    apply InEnv_insert_n. assumption.
+   destruct (lt_dec x v).
+   inversion Hsub.
+   assert (v = S v0) as HvSv0. destruct v. omega. subst. simpl. rewrite <- minus_n_O. reflexivity.
+   rewrite HvSv0.
+   apply get_insert_ge. rewrite H. assumption.
+   omega.
+  apply get_insert_lt. inversion Hsub. assumption. omega.
+
+ inversion Hsub. constructor.
+ inversion Hsub. constructor.
+ rewrite <- uninsert.
+ eapply IHe'.
+ eassumption.
+ apply weakening_cons.
+ assumption.
+ simpl; omega.
+
+ inversion Hsub; subst; eapply ty_app.
+ eapply IHe'1; eassumption.
+ eapply IHe'2; eassumption.
+Qed.
+
+
+Inductive val : Exp -> Prop :=
+  | v_num n : val (num n)
+  | v_lambda t b : val (lambda t b).
+
+Inductive e_step : Exp -> Exp -> Prop :=
+  | e_app1 e1 e1' e2 : e_step e1 e1' -> e_step (app e1 e2) (app e1' e2)
+  | e_app2 e1 e2 e2' : val e1 -> e_step e2 e2' -> e_step (app e1 e2) (app e1 e2')
+  | e_lam  t b x     : val x -> e_step (app (lambda t b) x) (subst b x 0).
+
+
+Lemma preservation e e' t:
+      TYPE [] e t ->
+      e_step e e' ->
+      TYPE [] e' t.
+Proof.
+ intros Ht He.
+ revert t Ht.
+ induction He; intros; inversion Ht; subst;
+ try econstructor; try apply IHHe; try eassumption.
+ inversion H2;
+ eapply substitution;
+ eassumption.
+Qed.
+
+
+Lemma progress e t:
+      TYPE [] e t ->
+      val e \/ (exists e', e_step e e').
+Proof.
+ intros Ht.
+ remember [] as ENV.
+ induction Ht; try solve [left; constructor].
+ subst. apply not_InEnv_nil in H. destruct H.
+ right.
+  destruct IHHt1. assumption.
+  destruct IHHt2. assumption.
+  inversion H; subst; inversion Ht1; subst.
+  eexists. eapply e_lam. assumption.
+
+  destruct H0.
+  eexists. eapply e_app2; eassumption.
+
+  destruct H.
+  eexists. eapply e_app1; eassumption.
+Qed.
+
+
+Inductive bigstep: Exp -> Exp -> Prop :=
+  | b_num n    : bigstep (num n) (num n)
+  | b_lam t b  : bigstep (lambda t b) (lambda t b)
+  | b_app f t b x x' v :
+        bigstep f (lambda t b)   ->
+        bigstep x x'             ->
+        bigstep (subst b x' 0) v ->
+        bigstep (app f x) v.
+
+Definition tc := transitive_closure Exp e_step.
+
+Lemma bigstep__val e v:
+      bigstep e v -> val v.
+Proof.
+ intros. induction H; try constructor; try assumption.
+Qed.
+
+Lemma e_step_noval e e':
+      e_step e e' ->
+      ~ val e.
+Proof.
+ intros H Hv.
+ induction Hv;
+ inversion H.
+Qed.
+
+Lemma e_step_deterministic e e' e'':
+      e_step e e'  ->
+      e_step e e'' ->
+      e' = e''.
+ intros He1 He2.
+ revert e'' He2.
+ induction He1; intros.
+ inversion He2; subst.
+
+ replace e1' with e1'0 in *.
+  reflexivity. symmetry. apply IHHe1. assumption.
+ eapply e_step_noval in H1. destruct H1.
+ eassumption.
+
+ inversion He1.
+
+ inversion He2; subst.
+ eapply e_step_noval in H. destruct H. eassumption.
+ apply IHHe1 in H4. rewrite H4. reflexivity.
+
+ eapply e_step_noval in H3. destruct H3. eassumption.
+
+ inversion He2; subst.
+ inversion H3.
+ eapply e_step_noval in H. destruct H. eassumption.
+ reflexivity.
+Qed.
+
+ 
+
+
+Lemma tc_app t b s s' v:
+      tc (app (lambda t b) s) v ->
+      tc s s' ->
+      val v   ->
+      tc (app (lambda t b) s') v.
+Proof.
+ intros Ha Hs Hv.
+ revert t b v Ha Hv.
+ induction Hs; intros; subst.
+ assumption.
+ apply IHHs.
+ inversion Ha; subst.
+ inversion Hv.
+ inversion H0; subst.
+ inversion H5.
+ replace e2' with s' in *.
+ eassumption.
+ eapply e_step_deterministic; eassumption.
+
+ eapply e_step_noval in H6. destruct H6. eassumption.
+ assumption.
+Qed.
+  
+
+
+Lemma tc_app2 t b s s' v:
+      tc (app (lambda t b) s') v ->
+      tc s s' ->
+      val v   ->
+      tc (app (lambda t b) s) v.
+Proof.
+ intros Ha Hs Hv.
+ revert t b v Ha Hv.
+ induction Hs; intros; subst.
+ assumption.
+ eapply tc_step. apply e_app2. constructor. eassumption.
+ apply IHHs; assumption.
+Qed.
+
+
+Lemma tc_app1 e1 e1' e2 v:
+      tc (app e1' e2) v ->
+      tc e1 e1' ->
+      tc (app e1 e2) v.
+Proof.
+ intros Ha Hs.
+ revert e2 v Ha.
+ induction Hs; intros; subst.
+ assumption.
+ eapply tc_step. apply e_app1. eassumption.
+ apply IHHs; assumption.
+Qed.
+
+(* H0 : bigstep x x'
+H1 : bigstep (subst b x' 0) v
+IHbigstep2 : tc x x'
+IHbigstep3 : tc (subst b x' 0) v
+H : bigstep (lambda t b) (lambda t b)
+IHbigstep1 : tc (lambda t b) (lambda t b)
+s' : Exp
+H2 : e_step x s'
+H3 : transitive_closure Exp e_step s' x'
+______________________________________(1/3)
+transitive_closure Exp e_step (app (lambda t b) s') v
+*)
+
+Lemma bigstep__e_step e v:
+      bigstep e v ->
+      tc e v.
+Proof.
+ intros. induction H; try constructor.
+ eapply tc_concat.
+  inversion IHbigstep1; subst.
+   inversion IHbigstep2; subst.
+   eapply tc_step. eapply e_lam. eapply bigstep__val; eassumption.
+  eassumption.
+   eapply tc_step. eapply e_app2; try constructor; eassumption.
+
+   inversion H3; subst.
+    eapply tc_step. eapply e_lam. eapply bigstep__val. eassumption.
+    assumption.
+
+   
+
+   eapply tc_app2 with (s' := x').
+    eapply tc_step. eapply e_lam.
+    eapply bigstep__val. eassumption.
+    assumption. assumption.
+    eapply bigstep__val; eassumption.
+
+
+   eapply tc_app1 with (e1' := lambda t b).
+    eapply tc_app2 with (s' := x').
+     eapply tc_step. eapply e_lam. eapply bigstep__val; eassumption.
+     assumption.
+     assumption.
+    eapply bigstep__val; eassumption.
+    eassumption.
+
+ apply tc_refl.
+Qed.
+
+Lemma val__bigstep v:
+      val v ->
+      bigstep v v.
+Proof.
+ intros Hv.
+ destruct Hv; constructor.
+Qed.
+
+Lemma e_step__bigstep e e' v:
+      e_step e e'  ->
+      bigstep e' v ->
+      bigstep e  v.
+Proof.
+ intros He Hbs.
+ revert v Hbs.
+ induction He; intros.
+ inversion Hbs; subst.
+ eapply b_app.
+ apply IHHe; eassumption.
+ eassumption.
+ assumption.
+
+ inversion Hbs; subst.
+ eapply b_app; try eassumption.
+ eapply IHHe; eassumption.
+
+ apply val__bigstep in H.
+ eapply b_app; try constructor; try eassumption.
+Qed.
 
