PFPL/TransitiveClosure.v
@@ -1,0 +1,47 @@
+
+Inductive transitive_closure (S : Type) (step : S -> S -> Type) : S -> S -> Prop :=
+  | tc_refl (s : S) : transitive_closure S step s s
+  | tc_step (s s' s'' : S) :
+            step s s' ->
+            transitive_closure S step s' s'' ->
+            transitive_closure S step s  s''.
+
+Inductive n_steps (St : Type) (step : St -> St -> Type) : nat -> St -> St -> Prop :=
+  | n_s_0   (s : St) : n_steps St step 0 s s
+  | n_s_S   (s s' s'' : St) (n : nat) :
+            step s s' ->
+            n_steps St step n s' s'' ->
+            n_steps St step (S n) s  s''.
+
+
+Theorem tc__n_steps St step s s' :
+        transitive_closure St step s s' <->
+        exists k, n_steps St step k s s'.
+Proof.
+ split; intros.
+  induction H.
+   exists 0; constructor.
+   destruct IHtransitive_closure.
+   exists (S x). eapply n_s_S; eassumption.
+  destruct H.
+  induction H.
+   constructor.
+   econstructor; eassumption.
+Qed.
+
+
+Lemma tc_concat {E S} e1 e2 e3:
+      transitive_closure E S e1 e2 ->
+      transitive_closure E S e2 e3 ->
+      transitive_closure E S e1 e3.
+Proof.
+ intros H1 H2.
+ revert e3 H2.
+ induction H1; intros.
+ assumption.
+ eapply tc_step.
+ eassumption.
+ apply IHtransitive_closure.
+ assumption.
+Qed.
+
